@prefix schema: <http://schema.org/> .
@prefix : <http://km.blackswantechnologies.ai/element/voc/km#> .
@prefix grddl: <http://www.w3.org/2003/g/data-view#> .
@prefix bst: <http://km.blackswantechnologies.ai/element/resource/> .
@prefix owl: <http://www.w3.org/2002/07/owl#> .
@prefix clientresource: <http://km.blackswantechnologies.ai/element/custom/> .
@prefix dkm: <http://blackswantechnologies.ai/element/km/dkm/> .
@prefix xsd: <http://www.w3.org/2001/XMLSchema#> .
@prefix fn: <http://www.w3.org/2005/xpath-functions#> .
@prefix skos: <http://www.w3.org/2004/02/skos/core#> .
@prefix rdfs: <http://www.w3.org/2000/01/rdf-schema#> .
@prefix sys: <http://www.ontotext.com/owlim/system#> .
@prefix ns1: <http://km.blackswantechnologies.ai/element/voc/> .
@prefix path: <http://www.ontotext.com/path#> .
@prefix ns5: <http://km.blackswantechnologies.ai/element/resource/tag/> .
@prefix kmt: <http://km.blackswantechnologies.ai/element/term/> .
@prefix dct: <http://purl.org/dc/terms/> .
@prefix vann: <http://purl.org/vocab/vann/> .
@prefix dcat: <http://www.w3.org/ns/dcat#> .
@prefix map: <http://blackswantechnologies.ai/element/km/mapping/> .
@prefix rdf4j: <http://rdf4j.org/schema/rdf4j#> .
@prefix wgs: <http://www.w3.org/2003/01/geo/wgs84_pos#> .
@prefix gn: <http://www.geonames.org/ontology#> .
@prefix vocabor: <http://km.blackswantechnologies.ai/element/voc/or#> .
@prefix rdf: <http://www.w3.org/1999/02/22-rdf-syntax-ns#> .
@prefix kgdata: <http://km.blackswantechnologies.ai/element/resource/data/> .
@prefix x: <http://km.blackswantechnologies.ai/element/test#> .
@prefix sesame: <http://www.openrdf.org/schema/sesame#> .
@prefix luc: <http://www.ontotext.com/owlim/lucene#> .
@prefix dc: <http://purl.org/dc/elements/1.1/> .

xsd:string a rdfs:Datatype, :DataType;
  rdfs:comment "Sequence of characters"@en;
  rdfs:label "String"@en .

xsd:integer a rdfs:Datatype, :DataType;
  rdfs:comment "Integer value with range -N to N numeral value"@en;
  rdfs:label "Integer"@en .

:ParamMapping a owl:Class;
  rdfs:subClassOf :Mapping, _:genid-6746439800084d48b9df2105733e82b8-2FB2112B4CD459A620A61D4F4C9EFD34,
    _:genid-6746439800084d48b9df2105733e82b8-4B3BF59C37C21E83A64E0F4B77D91030;
  rdfs:comment "An association between a query parameter and an attribute containig the value to be instantiated. "@en;
  rdfs:label "Parameter mapping"@en .

:fetcherQueryParam a owl:DatatypeProperty;
  rdfs:comment "The name of a parameter used in a fetcher query."@en;
  rdfs:label "fetcher query parameter"@en;
  schema:domainIncludes :ParamMapping;
  schema:rangeIncludes xsd:string .

:AttributeType a owl:Class;
  rdfs:subClassOf :PropertyType, _:genid-6746439800084d48b9df2105733e82b8-5BC5CB2EA85992929A61F7BDF2256141,
    _:genid-6746439800084d48b9df2105733e82b8-2E9D3F7137F6A76B94974B7D76BF70F2, _:genid-6746439800084d48b9df2105733e82b8-9746471FEBD076D53A5C77C697CBF4EC,
    _:genid-6746439800084d48b9df2105733e82b8-382D61534EC133EFF603D88BCD44FF81;
  rdfs:comment "A property type associating a term with a literal data value (a scalar) of specific data type"@en,
    "In OWL representation, relationship types correspond to all explicitly defined instances of owl:DatatypeProperty."@en;
  rdfs:label "Attribute type"@en .

:hasDomain a owl:ObjectProperty;
  rdfs:comment "Indicates the types included in the domain of the property."@en;
  rdfs:label "has domain"@en;
  schema:domainIncludes :PropertyType;
  schema:rangeIncludes :EntityType, :RelationshipType .

:hasRange a owl:ObjectProperty;
  rdfs:comment "Associates a property with its range type."@en, "This property should not be used directly when defining a DKM ontology."@en;
  rdfs:label "has range"@en;
  schema:domainIncludes :PropertyType;
  schema:rangeIncludes :Term .

:Application a owl:Class;
  rdfs:subClassOf owl:Thing, _:genid-6746439800084d48b9df2105733e82b8-11DEA6DD7E1795BBC455ED9F217BC4C0,
    _:genid-6746439800084d48b9df2105733e82b8-6D476D0F703404CEEFE0C18B304653F2, _:genid-6746439800084d48b9df2105733e82b8-49088FF45F25F3F99770047F6B347E2D;
  rdfs:comment "A KG-based application developed by a customer."@en;
  rdfs:label "Application"@en .

:hasDataSource a owl:ObjectProperty;
  rdfs:comment "Associates data source configuration used by the application."@en;
  rdfs:label "has data source"@en;
  schema:domainIncludes :Application;
  schema:rangeIncludes :DataSourceConfig .

:hasOwner a owl:ObjectProperty;
  rdfs:comment "Associates an Owner(Agent) with the owned resources(Application, DataSource, DataMapping)"@en;
  rdfs:label "has owner"@en;
  schema:domainIncludes :Application, :Fetcher, :DataMapping, :DataSource;
  schema:rangeIncludes :Agent .

:hasSchema a owl:ObjectProperty;
  rdfs:comment "The schema of the application."@en;
  rdfs:label "has schema"@en;
  schema:domainIncludes :Application;
  schema:rangeIncludes :AppSchema .

:credibility a owl:DatatypeProperty;
  rdfs:comment "Credibility for attribute."@en;
  rdfs:label "credibility"@en;
  schema:domainIncludes :AttributeCredibility;
  schema:rangeIncludes xsd:decimal .

:description a owl:DatatypeProperty;
  rdfs:comment "An informative description of the resource."@en;
  rdfs:label "description"@en;
  schema:domainIncludes :Domain, :DataSource;
  schema:rangeIncludes xsd:string .

:Domain a owl:Class;
  rdfs:subClassOf owl:Thing, _:genid-6746439800084d48b9df2105733e82b8-4405AEBBDF958CEF1E7708B241281AEE,
    _:genid-6746439800084d48b9df2105733e82b8-58D6840799894E91E9D5833215590993, _:genid-6746439800084d48b9df2105733e82b8-87C9B026CF224FFE9F5E2FDA1DB42F75,
    _:genid-6746439800084d48b9df2105733e82b8-72DBE3ECD38BD00C9AB4E27BBFAD54A2;
  rdfs:comment "A (knowledge mesh) application domain such as Organization Research, Cyber Security, Healthcare, Logistics, etc."@en;
  rdfs:label "Domain"@en .

:hasCatalog a owl:ObjectProperty;
  rdfs:comment "The data catalog describing data sources associated with the domain."@en;
  rdfs:label "has catalog"@en;
  schema:domainIncludes :Domain;
  schema:rangeIncludes :Catalog .

:hasDKM a owl:ObjectProperty;
  rdfs:comment "The domain knolwedge model associated with the domain."@en;
  rdfs:label "has DKM"@en;
  schema:domainIncludes :Domain;
  schema:rangeIncludes :DKM .

:Agent a owl:Class;
  rdfs:subClassOf owl:Thing, _:genid-6746439800084d48b9df2105733e82b8-D11091805A807977944BCA0DB69B4C83;
  rdfs:comment "Any subject appearing as an asset owner or tenant within KM (e.g. dataset owner, application creator, etc.)."@en;
  rdfs:label "Agent"@en .

:AppSchema a owl:Class;
  rdfs:subClassOf :KGSchema, _:genid-6746439800084d48b9df2105733e82b8-D639C7E3DA9990504771C273B2958348,
    _:genid-6746439800084d48b9df2105733e82b8-08AD7611C7ACAB54A6FD10D3820062E4;
  rdfs:comment "A KG schema of an application."@en;
  rdfs:label "Application schema"@en .

:containsTerm a owl:ObjectProperty;
  rdfs:comment "A vocabulary contains a specific term. This property, though in principle redundant, can be usefuly surfaced in order to facilitate  analysis of semantic connections between different vocabularies, or vocabularies and sources. "@en;
  rdfs:label "contains term"@en;
  schema:domainIncludes :Vocabulary;
  schema:rangeIncludes :Term .

:Fetcher a owl:Class;
  rdfs:subClassOf owl:Thing, _:genid-6746439800084d48b9df2105733e82b8-7889BA61DF817F3F77DFA7ED239C51BC,
    _:genid-6746439800084d48b9df2105733e82b8-CB920E82075E905CFE466DCDE62707D7, _:genid-6746439800084d48b9df2105733e82b8-4805876D8198EFD31220D0C776C766B2,
    _:genid-6746439800084d48b9df2105733e82b8-60274FBC857B96C997097A6B734DB8B7, _:genid-6746439800084d48b9df2105733e82b8-1CEBA1321A0DC87AAE75E5731D08E463,
    _:genid-6746439800084d48b9df2105733e82b8-083164EC1D5A7192C343F2E5092C2AF4, _:genid-6746439800084d48b9df2105733e82b8-9197CED36C10EF78061BF49136C19BD6;
  rdfs:comment "A service providing access to a dataset. It exposes some data querying interface and serves results in a specific format."@en;
  rdfs:label "Fetcher"@en .

:serves a owl:ObjectProperty;
  rdfs:comment "Data source served by the fetcher."@en;
  rdfs:label "serves data source"@en;
  schema:domainIncludes :Fetcher;
  schema:rangeIncludes :DataSource .

:DataMapping a owl:Class;
  rdfs:subClassOf :DataOperation, :Mapping, _:genid-6746439800084d48b9df2105733e82b8-0837DACF01C925857341BD806B158E86,
    _:genid-6746439800084d48b9df2105733e82b8-F1DB545944643BE6171516CCF3C1E0DB, _:genid-6746439800084d48b9df2105733e82b8-DCC3D109A58A156AE0D95D2154E0402C,
    _:genid-6746439800084d48b9df2105733e82b8-9F6026F57AD5C848E93F596D266B1946;
  rdfs:comment "A mapping of a data source to a DKM vocabulary."@en;
  rdfs:label "Data mapping"@en .

:fetcherQuery a owl:DatatypeProperty;
  rdfs:comment "GraphQL query used by the mapping for sourcing required data."@en;
  rdfs:label "fetcher query"@en;
  schema:domainIncludes :DataMapping;
  schema:rangeIncludes xsd:string .

:queryParamMapping a owl:ObjectProperty;
  rdfs:comment "Association between an attribute whose values are used to instantiate fetcher query parameter and that parameter. "@en;
  rdfs:label "query parameter mapping"@en;
  schema:domainIncludes :DataMapping;
  schema:rangeIncludes :ParamMapping .

:sourceFetcher a owl:ObjectProperty;
  rdfs:comment "The fetcher serving data mapped by the data mapping. "@en;
  rdfs:label "source fetcher"@en;
  schema:domainIncludes :DataMapping;
  schema:rangeIncludes :Fetcher .

:targetTerm a owl:ObjectProperty;
  rdfs:comment "The term from the target vocabulary referred to from the mapping. In case of the :TermMapping this is a term to which the source term is mapped. For :DataMapping it's one of the DKM terms that might be mentioned in the mapping.."@en;
  rdfs:label "target term"@en;
  schema:domainIncludes :DataMapping, :TermMapping;
  schema:rangeIncludes :Term .

:SparqlQuery a owl:Class;
  rdfs:subClassOf owl:Thing, _:genid-6746439800084d48b9df2105733e82b8-A377FED1B36A9F10C98F4CDA786715EB;
  rdfs:comment "An object encoding a SPARQL query, possibly using alternative serializations. "@en;
  rdfs:label "SPARQL query"@en .

:queryString a owl:DatatypeProperty;
  rdfs:comment "SPARQL query used with data mapping"@en;
  rdfs:label "query string"@en;
  schema:domainIncludes :SparqlQuery, :ValidationConstraint;
  schema:rangeIncludes xsd:string .

:EntityType a owl:Class;
  rdfs:subClassOf :Term;
  rdfs:comment "A type of entities (or other auxiliary modeling objects)"@en, "In OWL representation, entity types correspond to all explicitly defined instances of owl:Class, subclasses of owl:Thing."@en;
  rdfs:label "Entity type"@en .

:DataSource a owl:Class;
  rdfs:subClassOf owl:Thing, _:genid-6746439800084d48b9df2105733e82b8-7889BA61DF817F3F77DFA7ED239C51BC,
    _:genid-6746439800084d48b9df2105733e82b8-599DAF6E1ECB4035C86ABF6DD80392AF, _:genid-6746439800084d48b9df2105733e82b8-E4BFC45CCB15A51C1256CAED5FEE6199,
    _:genid-6746439800084d48b9df2105733e82b8-B2DE942CCE1B3BE4D2CAFF4B0C3F6DF6, _:genid-6746439800084d48b9df2105733e82b8-18219C53B0393C2DEA8647CCAFC74E8C,
    _:genid-6746439800084d48b9df2105733e82b8-C4BD601677F153FEA84A8FA729D66EC9;
  rdfs:comment "A collection of data resources available for consumption for KM applications."@en;
  rdfs:label "Data source"@en .

:website a owl:DatatypeProperty;
  rdfs:comment "The home page URL of the resource"@en;
  rdfs:label "website"@en;
  schema:domainIncludes :DataSource;
  schema:rangeIncludes xsd:anyURI .

xsd:boolean a rdfs:Datatype, :DataType;
  rdfs:comment "Possible values: true | false"@en;
  rdfs:label "Boolean"@en .

:Catalog a owl:Class;
  rdfs:subClassOf owl:Thing, _:genid-6746439800084d48b9df2105733e82b8-F5CAC69CB0E4B3CFF7A6980E483298A0;
  rdfs:comment "A collection of metadata records representing a collection of datasets."@en;
  rdfs:label "Data catalog"@en .

:containsDataSource a owl:ObjectProperty;
  rdfs:comment "A data source contained in a data catalog."@en;
  rdfs:label "contains data source"@en;
  schema:domainIncludes :Catalog;
  schema:rangeIncludes :DataSource .

:DKM a owl:Class;
  rdfs:subClassOf :KGSchema;
  rdfs:comment "Default KG schema for a KM domain."@en;
  rdfs:label "Domain knowledge model"@en .

:endpointURL a owl:DatatypeProperty;
  rdfs:comment "The URL of a query endpoint exposing some data resources (typically endpoint of a fetcher)."@en;
  rdfs:label "endpoint URL"@en;
  schema:domainIncludes :Fetcher;
  schema:rangeIncludes xsd:anyURI .

:targetDomain a owl:ObjectProperty;
  rdfs:comment "The target domain of the data mapping."@en;
  rdfs:label "target domain"@en;
  schema:domainIncludes :DataMapping;
  schema:rangeIncludes :Domain .

:RelationshipType a owl:Class;
  rdfs:subClassOf :PropertyType;
  rdfs:comment "A property type relating two entities of specific types"@en, "In OWL representation, relationship types correspond to all explicitly defined instances of owl:ObjectProperty."@en;
  rdfs:label "Relationship type"@en .

:PropertyType a owl:Class;
  rdfs:subClassOf :Term, _:genid-6746439800084d48b9df2105733e82b8-00F064439EC626D99F909E28643CC94E,
    _:genid-6746439800084d48b9df2105733e82b8-02A0499502B45FD7003F68DE85CF9E85;
  rdfs:comment "DKM properties include: relationship types and attribute types."@en;
  rdfs:label "Property type"@en .

:Term a owl:Class;
  rdfs:subClassOf owl:Thing, _:genid-6746439800084d48b9df2105733e82b8-08AD7611C7ACAB54A6FD10D3820062E4,
    _:genid-6746439800084d48b9df2105733e82b8-F4DEE88442E4A64EE808B149579972F9;
  rdfs:comment "A DKM modeling term, being one of: entity type, relationship type, attribute type, data type, taxonomy concept ."@en;
  rdfs:label "Term"@en .

:referenceTerm a owl:ObjectProperty;
  rdfs:comment "Application term references a domain term, meaning that the it originates from the latter (e.g. by import) and is semantically equivalent."@en;
  rdfs:label "reference term"@en;
  schema:domainIncludes :Term;
  schema:rangeIncludes :Term .

xsd:decimal a rdfs:Datatype, :DataType;
  rdfs:comment "Decimal data type used across credibility/dataValidityPeriodInHours etc."@en;
  rdfs:label "Decimal"@en .

:referenceSource a owl:ObjectProperty;
  rdfs:comment "Application data source references another source, meaning that it originates from that latter source (e.g. by import) and is technically the same resource just used in a dfierent role."@en;
  rdfs:label "reference source"@en;
  schema:domainIncludes :DataSourceConfig;
  schema:rangeIncludes :DataSource .

xsd:anyURI a rdfs:Datatype, :DataType;
  rdfs:comment "Uniform Resource Identifier Reference (URI) used to restrict values to http/https links"@en;
  rdfs:label "URI"@en .

:TermMapping a owl:Class;
  rdfs:subClassOf :Mapping;
  rdfs:comment "Specification of a match between a DKM term (source) and some semantically related, external vocabulary term (target)."@en;
  rdfs:label "Term mapping"@en .

:mappingRule a owl:ObjectProperty;
  rdfs:comment "Mapping rule contained in the data mapping."@en;
  rdfs:label "mapping rule"@en;
  schema:domainIncludes :DataMapping;
  schema:rangeIncludes :SparqlQuery .

:paramValueAttribute a owl:ObjectProperty;
  rdfs:comment "Attribute being the source of values for instantiating the parameter."@en;
  rdfs:label "parameter value attribute"@en;
  schema:domainIncludes :ParamMapping;
  schema:rangeIncludes :AttributeType .

ns1:km a owl:Ontology;
  rdfs:comment "The core vocabulary for representing the ELEMENT Knowledge Mesh architecture. (Resources having ScopeNotes as MVP are under scope of this release. Kindly ignore resources having ScopeNotes as non-MVP-related.)"@en;
  rdfs:label "The ELEMENT Knowledge Mesh Core Ontology"@en;
  rdfs:seeAlso "https://blackswantechnologies.atlassian.net/wiki/spaces/KMA/pages/3311796301/Knowledge+Mesh+Core+Ontology" .

:KGSchema a owl:Class;
  rdfs:subClassOf :Ontology, _:genid-6746439800084d48b9df2105733e82b8-95B9566C26265D611AD436E2EF19B40B;
  rdfs:comment "A knowledge graph schema defined as a collection of interconnected terms (entity, relationship and attribute types)."@en;
  rdfs:label "Knowledge Graph schema"@en .

:Ontology a owl:Class;
  rdfs:subClassOf owl:Ontology, :Vocabulary;
  rdfs:comment "Ontology represented in KM Metadata"@en;
  rdfs:label "Ontology"@en .

:Attribute a owl:Class;
  rdfs:subClassOf :Instance;
  rdfs:comment "A reified subject-attribute-value statement. An instance of an attribute."@en;
  rdfs:label "Attribute"@en .

:Instance a owl:Class;
  rdfs:subClassOf owl:Thing;
  rdfs:comment "A data instance of a certain type. An individual, data-level component of a knowledge graph."@en;
  rdfs:label "Data instance"@en .

:AttributeMatcher a owl:Class;
  rdfs:subClassOf owl:Thing, _:genid-6746439800084d48b9df2105733e82b8-F5CAC69CB0E4B3CFF7A6980E483298A0,
    _:genid-6746439800084d48b9df2105733e82b8-7371238C9EF20336A05A02C33FC95E25, _:genid-6746439800084d48b9df2105733e82b8-ED6291985F77CB59B973D4E81D3F1D9A;
  rdfs:comment "An implementation of a method for calculating similarity between values of a specific attribute."@en;
  rdfs:label "Attribute matcher"@en .

:Concept a owl:Class;
  rdfs:subClassOf :Term;
  rdfs:comment "A (taxonomy) concept can be viewed as an idea or notion; a unit of thought. However, what constitutes a unit of thought is subjective, and this definition is meant to be suggestive, rather than restrictive."@en;
  rdfs:label "Concept"@en .

:DataDeployment a owl:Class;
  rdfs:subClassOf :DataOperation;
  rdfs:comment "Operation to get deployed data"@en;
  rdfs:label "Data deployment"@en .

:DataOperation a owl:Class;
  rdfs:subClassOf owl:Thing;
  rdfs:comment "A collection of operations on data - retrieval/inference/validation etc"@en;
  rdfs:label "Data operation"@en .

:DataInference a owl:Class;
  rdfs:subClassOf :DataOperation;
  rdfs:comment "Operation to get Inferred data"@en;
  rdfs:label "Data inference"@en .

:Mapping a owl:Class;
  rdfs:subClassOf owl:Thing;
  rdfs:comment "A formal specification of a mapping of data/vocabulary (source) to a vocabulary (target). An abstraction class over different types of mapping formalizations."@en,
    "The required URI pattern for instances of this type is: http://blackswantechnologies.ai/element/km/mapping/, where ID is preferably a UUID or other unique randomly generated string."@en;
  rdfs:label "Mapping"@en .

:DataRetrieval a owl:Class;
  rdfs:subClassOf :DataOperation;
  rdfs:comment "Data Retrieval operation"@en;
  rdfs:label "Data retrieval"@en .

:DataType a owl:Class;
  rdfs:subClassOf rdfs:Datatype, :Term;
  rdfs:comment "A set of literals (scalar values) of certain type, such as strings, integers, dates"@en,
    "The set of permitted data types is pre-defined and corresponds to selected XML data type (https://www.w3.org/TR/xmlschema11-2)"@en;
  rdfs:label "Data type"@en;
  rdfs:isDefinedBy "https://www.w3.org/TR/xmlschema11-2"^^xsd:anyURI .

:DataValidation a owl:Class;
  rdfs:subClassOf :DataOperation;
  rdfs:comment "Operation for validating data"@en;
  rdfs:label "Data validation"@en .

:Entity a owl:Class;
  rdfs:subClassOf :Instance;
  rdfs:comment "An entity (an individual domain object). An instance of some entity type."@en;
  rdfs:label "Entity"@en .

:Enumeration a owl:Class;
  rdfs:subClassOf owl:Thing;
  rdfs:comment "Enumeration of items (depending on the context expressed as a skos:ConceptScheme or an owl:Class of instances)."@en;
  rdfs:label "Enumeration"@en .

:Vocabulary a owl:Class;
  rdfs:subClassOf owl:Thing;
  rdfs:comment "Any formal semantic model defining some domain terminology (e.g. ontologies, taxonomies, thesauri, controlled vocabularies, schemas, etc.)"@en;
  rdfs:label "Vocabulary"@en .

:MappingSKOS a owl:Class;
  rdfs:subClassOf :TermMapping;
  rdfs:comment "Term mapping following the SKOS semantics of match relationships"@en;
  rdfs:label "SKOS mapping"@en;
  rdfs:seeAlso "https://www.w3.org/TR/skos-reference/#mapping"^^xsd:anyURI .

:Relationship a owl:Class;
  rdfs:subClassOf :Instance;
  rdfs:comment "A reified subject-relationship-object statement. An instance of some relationship type. "@en;
  rdfs:label "Relationship"@en .

:Taxonomy a owl:Class;
  rdfs:subClassOf :Vocabulary, skos:ConceptScheme;
  rdfs:comment "Taxonomy represented in KM Metadata"@en;
  rdfs:label "Taxonomy"@en .

:describedBy a owl:ObjectProperty;
  rdfs:comment "Data in a specific source is described by a DKM term or the data source as a whole is described by some term."@en;
  rdfs:label "described by"@en;
  schema:domainIncludes :DataSource;
  schema:rangeIncludes :Term .

:enumerable a owl:DatatypeProperty;
  rdfs:comment "Indicates whether attribute type is enumerable (ranges over a finite set of values) or not. "@en;
  rdfs:label "is enumerable"@en;
  schema:domainIncludes :AttributeType;
  schema:rangeIncludes xsd:boolean .

:enumeratedValues a owl:ObjectProperty;
  rdfs:comment "Indicates that the property must take one of the enumerated values."@en;
  rdfs:label "enumerated values"@en;
  schema:domainIncludes :PropertyType;
  schema:rangeIncludes :Enumeration .

:extractedLabel a owl:DatatypeProperty;
  rdfs:comment "Any (correct or incorrect) concept label that can be encountered in actual data and associated with that concept. "@en;
  rdfs:label "extracted label"@en;
  schema:domainIncludes :Concept;
  schema:rangeIncludes xsd:string .

:from a owl:ObjectProperty;
  rdfs:subPropertyOf :relationshipComponent;
  rdfs:comment "Indicates the entity at the subject position of the relationship, e.g. :mary in <:mary :likes :bill>."@en;
  rdfs:label "from"@en;
  schema:domainIncludes :Relationship;
  schema:rangeIncludes :Entity .

:relationshipComponent a owl:ObjectProperty;
  rdfs:comment "Abstraction over relationship component properties, used for representing reified relationships."@en;
  rdfs:label "relationship component"@en;
  schema:domainIncludes :Relationship;
  schema:rangeIncludes :Entity .

:hasDataRange a owl:ObjectProperty;
  rdfs:subPropertyOf :hasRange;
  rdfs:comment "Associates a relationship with data types of its allowed values."@en;
  rdfs:label "has data range"@en;
  schema:domainIncludes :AttributeType;
  schema:rangeIncludes :DataType .

:hasEntityRange a owl:ObjectProperty;
  rdfs:subPropertyOf :hasRange;
  rdfs:comment "Associates a relationship with entity types of its allowed values."@en;
  rdfs:label "has entity range"@en;
  schema:domainIncludes :RelationshipType;
  schema:rangeIncludes :EntityType .

:hasMatch a owl:ObjectProperty;
  owl:inverseOf :sourceTerm;
  rdfs:comment "A mapping to a term from an external vocabulary"@en, "See the description of mv:Mapping, mv:targetVocabulary, mv:targetTerm for further details."@en;
  rdfs:label "has match"@en;
  schema:domainIncludes :Term;
  schema:rangeIncludes :MappingSKOS .

:sourceTerm a owl:ObjectProperty;
  owl:inverseOf :hasMatch;
  rdfs:comment "The DKM term that has a matching term in an external vocabulary"@en;
  rdfs:label "source term"@en;
  schema:domainIncludes :TermMapping;
  schema:rangeIncludes :Term .

:hasProperty a owl:ObjectProperty;
  owl:inverseOf :hasDomain;
  rdfs:comment "Associates a class with its allowed properties; alternatively, indicates the classes included in the domain of the property."@en;
  rdfs:label "has property"@en;
  schema:domainIncludes :Term;
  schema:rangeIncludes :PropertyType .

:matchType a owl:ObjectProperty;
  rdfs:comment "The assumed default (in case the value is missing) is http://www.w3.org/2004/02/skos/core#exactMatch"@en,
    "The type of match assumed in the mapping - preferably one of the SKOS mapping relation URIs (https://www.w3.org/TR/skos-reference/#mapping)."@en;
  rdfs:label "match type"@en;
  rdfs:isDefinedBy "https://www.w3.org/TR/skos-reference/#mapping"^^xsd:anyURI;
  schema:domainIncludes :MappingSKOS;
  schema:rangeIncludes owl:Thing .

:prefAbbreviation a owl:DatatypeProperty;
  rdfs:comment "BST-preferred abbreviation for some value"@en;
  rdfs:label "preferred abbreviation"@en;
  schema:domainIncludes :Concept;
  schema:rangeIncludes xsd:string .

:servedBy a owl:ObjectProperty;
  owl:inverseOf :serves;
  rdfs:comment "The fetcher that provides access to the data source."@en;
  rdfs:label "served by fetcher"@en;
  schema:domainIncludes :DataSource;
  schema:rangeIncludes :Fetcher .

:targetVocabulary a owl:ObjectProperty;
  rdfs:comment "Must be a URI uniquely identifying the vocabulary."@en, "The target vocabulary to which the term or data source is mapped. Might be an external/public vocabulary or a DKM."@en;
  rdfs:label "target vocabulary"@en;
  schema:domainIncludes :Mapping;
  schema:rangeIncludes owl:Thing .

:termScope a owl:DatatypeProperty;
  rdfs:comment "Some conventional value qualifying the scope of the term."@en;
  rdfs:label "term scope"@en;
  schema:domainIncludes :Term;
  schema:rangeIncludes xsd:string .

:to a owl:ObjectProperty;
  rdfs:subPropertyOf :relationshipComponent;
  rdfs:comment "Indicates the entity at the object position of the relationship, e.g. :bill in <:mary :likes :bill>.."@en;
  rdfs:label "to"@en;
  schema:domainIncludes :Relationship;
  schema:rangeIncludes :Entity .

:usesMatcher a owl:ObjectProperty;
  rdfs:comment "Matcher used by Attribute"@en;
  rdfs:label "uses matcher"@en;
  schema:domainIncludes :AttributeType;
  schema:rangeIncludes :AttributeMatcher .

xsd:date a rdfs:Datatype, :DataType;
  rdfs:comment "Pattern: YYYY-MM-DD"@en;
  rdfs:label "Date"@en .

xsd:dateTime a rdfs:Datatype, :DataType;
  rdfs:comment "Pattern YYYY-MM-DDThh:mm:ss[Z|(+|-)hh:mm]"@en;
  rdfs:label "Date-time"@en .

xsd:gYear a rdfs:Datatype, :DataType;
  rdfs:comment "Pattern: YYYY"@en;
  rdfs:label "Year"@en .

xsd:gYearMonth a rdfs:Datatype, :DataType;
  rdfs:comment "Pattern: YYYY-MM"@en;
  rdfs:label "Year-month"@en .

xsd:time a rdfs:Datatype, :DataType;
  rdfs:comment "time represents an instant of time that recurs every day"@en;
  rdfs:label "Time"@en .

:hasTag a owl:ObjectProperty;
  rdfs:comment "Property connecting Tag(key-value pair) associated with some KM Resource : Data-Source/Application Data-Source/ AppTerm"@en;
  rdfs:label "has tag"@en;
  schema:domainIncludes :EntityType, :DataSourceConfig;
  schema:rangeIncludes :Tag .

:Tag a owl:Class;
  rdfs:subClassOf owl:Thing, _:genid-6746439800084d48b9df2105733e82b8-65CDEC0784CC1FD612A5BD9E231F1E56,
    _:genid-6746439800084d48b9df2105733e82b8-15D00213FFE7ED7AC14AEE7217507503;
  rdfs:comment "Tag associated with some knowledge mesh resource - DataSource, DataMapping, Domain, Fetcher"@en;
  rdfs:label "Tag"@en .

:tagKey a owl:DatatypeProperty;
  rdfs:comment "Tag key is the key representing UI component (can be color, symbol)"@en;
  rdfs:label "tag key"@en;
  schema:domainIncludes :Tag;
  schema:rangeIncludes xsd:string .

:dataValidityPeriodInHours a owl:DatatypeProperty;
  rdfs:comment "Validity period for source data."@en;
  rdfs:label "data validity period"@en;
  schema:domainIncludes :DataSource;
  schema:rangeIncludes xsd:decimal .

:sourceMedium a owl:DatatypeProperty;
  rdfs:comment "Source medium for data source. values can be csv, fbe, gow, document"@en;
  rdfs:label "source medium"@en;
  schema:domainIncludes :DataSource;
  schema:rangeIncludes xsd:string .

:hasAttributeCredibility a owl:ObjectProperty;
  rdfs:comment "Credibility associated with a Data mapping"@en;
  rdfs:label "has attribute credibility"@en;
  schema:domainIncludes :DataMapping;
  schema:rangeIncludes :AttributeCredibility .

:AttributeCredibility a owl:Class;
  rdfs:subClassOf owl:Thing, _:genid-6746439800084d48b9df2105733e82b8-0B16489659A117A1E1002CF6235C797E,
    _:genid-6746439800084d48b9df2105733e82b8-2EEBDD89C16DE395ED765AFFFA896082;
  rdfs:comment "Credibility assigned to attribute type"@en;
  rdfs:label "Attribute credibility"@en .

:kgUsageCategory a owl:DatatypeProperty;
  rdfs:comment "Usage category for datasource : root/referance source"@en;
  rdfs:label "kg usage category"@en;
  schema:domainIncludes :DataSourceConfig;
  schema:rangeIncludes xsd:string .

:tagValue a owl:DatatypeProperty;
  rdfs:comment "Tag value is based on tag key"@en;
  rdfs:label "tag value"@en;
  schema:domainIncludes :Tag;
  schema:rangeIncludes xsd:string .

:responsePattern a owl:DatatypeProperty;
  rdfs:comment "Sync/Async type"@en;
  rdfs:label "response pattern"@en;
  schema:domainIncludes :Fetcher;
  schema:rangeIncludes xsd:string .

:maxParallelism a owl:DatatypeProperty;
  rdfs:comment "Parallelism upper limit on fetcher."@en;
  rdfs:label "max parallelism"@en;
  schema:domainIncludes :Fetcher;
  schema:rangeIncludes xsd:integer .

:paginationMode a owl:DatatypeProperty;
  rdfs:comment "Pagination mode for fetcher."@en;
  rdfs:label "pagination mode"@en;
  schema:domainIncludes :Fetcher;
  schema:rangeIncludes xsd:string .

:timeoutSeconds a owl:DatatypeProperty;
  rdfs:comment "Timeout on fetcher request (in seconds)."@en;
  rdfs:label "timeout seconds"@en;
  schema:domainIncludes :Fetcher;
  schema:rangeIncludes xsd:integer .

:overallCredibility a owl:DatatypeProperty;
  rdfs:comment "Combined Credibility Score for all attributes under specific data mapping."@en;
  rdfs:label "overall credibility"@en;
  schema:domainIncludes :DataMapping;
  schema:rangeIncludes xsd:decimal .

:hasAttribute a owl:ObjectProperty;
  rdfs:comment "Attribute credibility score associated with an Attribute."@en;
  rdfs:label "has attribute"@en;
  schema:domainIncludes :AttributeCredibility;
  schema:rangeIncludes :AttributeType .

:hasAppDomain a owl:ObjectProperty;
  rdfs:comment "Associates Application with Domain existing in KM."@en;
  rdfs:label "has application domain"@en;
  schema:domainIncludes :Application;
  schema:rangeIncludes :Domain .

:DataSourceConfig a owl:Class;
  rdfs:subClassOf owl:Thing, _:genid-6746439800084d48b9df2105733e82b8-06F3D36FB458C9B9E7FABBF9AC02C5FD,
    _:genid-6746439800084d48b9df2105733e82b8-61F8FBA8F30FFC8E0A12080541066628;
  rdfs:comment "An application-specific configuration of any data source."@en;
  rdfs:label "Data source configuration"@en .

:version a owl:DatatypeProperty;
  rdfs:comment "Application schema version."@en;
  rdfs:label "version"@en;
  schema:domainIncludes :AppSchema;
  schema:rangeIncludes xsd:string .

:cardinality a owl:DatatypeProperty;
  rdfs:comment "Cardinality for attribute."@en;
  rdfs:label "cardinality"@en;
  schema:domainIncludes :AttributeType;
  schema:rangeIncludes xsd:string .

:isMandatory a owl:DatatypeProperty;
  rdfs:comment "Attribute type is mandatory or not."@en;
  rdfs:label "is mandatory"@en;
  schema:domainIncludes :AttributeType;
  schema:rangeIncludes xsd:boolean .

:weight a owl:DatatypeProperty;
  rdfs:comment "Weight for attribute."@en;
  rdfs:label "weight"@en;
  schema:domainIncludes :AttributeType;
  schema:rangeIncludes xsd:decimal .

:ConstraintViolation a owl:Class;
  rdfs:subClassOf owl:Thing, _:genid-6746439800084d48b9df2105733e82b8-1AED1946F64D34E5E6D120CCF23E2983,
    _:genid-6746439800084d48b9df2105733e82b8-DB16376A000F45392A86C60D792C65C0, _:genid-6746439800084d48b9df2105733e82b8-535BEB1DC0EBB47191057BAA3DA7D606,
    _:genid-6746439800084d48b9df2105733e82b8-07FD9ADD00D292940971899CF952175B;
  rdfs:comment "Violation traced across a violating resource resulting from validation test."@en;
  rdfs:label "Constraint violation"@en .

:constraint a owl:ObjectProperty;
  rdfs:comment "URI of test suite for violation. Used as reference for information regarding a particular violation."@en;
  rdfs:label "constraint"@en;
  schema:domainIncludes :ConstraintViolation;
  schema:rangeIncludes :ValidationConstraint .

:ViolatingDataTrace a owl:Class;
  rdfs:subClassOf owl:Thing, _:genid-6746439800084d48b9df2105733e82b8-1AED1946F64D34E5E6D120CCF23E2983,
    _:genid-6746439800084d48b9df2105733e82b8-9E7542BA53AF77F7692A3F18B731D669, _:genid-6746439800084d48b9df2105733e82b8-A27BB97FFA10B3E76266C4A3EB38FCC4,
    _:genid-6746439800084d48b9df2105733e82b8-29B28C7FF7BBE4CF7213CEBA161202ED, _:genid-6746439800084d48b9df2105733e82b8-08F26CB98CC0FAB64C8B28FC490E134B,
    _:genid-6746439800084d48b9df2105733e82b8-489EB08BF2372314A349F48EB396FB4F, _:genid-6746439800084d48b9df2105733e82b8-BFB5A9BF98D939D3BDBAC7894F044580;
  rdfs:comment "A collection of violating resources resulting from failed validation tests."@en;
  rdfs:label "Violating data trace"@en .

:violatingData a owl:ObjectProperty;
  rdfs:comment "Associates constraint violation with violating data for tracing violation in Ontology or Data."@en;
  rdfs:label "violating data"@en;
  schema:domainIncludes :ConstraintViolation;
  schema:rangeIncludes :ViolatingDataTrace .

:inGraph a owl:ObjectProperty;
  rdfs:comment "Graph where violating data is traced after a failed validation test."@en;
  rdfs:label "constituent graph"@en;
  schema:domainIncludes :ConstraintViolation;
  schema:rangeIncludes rdfs:Resource .

:ValidationConstraint a owl:Class;
  rdfs:subClassOf owl:Thing, _:genid-6746439800084d48b9df2105733e82b8-8BFC629C1BA2ED077BD0164116ECA14B,
    _:genid-6746439800084d48b9df2105733e82b8-23C63E89CD7FE84E5A97DC2EF50F1946, _:genid-6746439800084d48b9df2105733e82b8-5AF5774FDED6F78E18507AECA5026364,
    _:genid-6746439800084d48b9df2105733e82b8-54BBD6EB4E58ADBB939DEB1EB4B920AD, _:genid-6746439800084d48b9df2105733e82b8-7131B58332CB5918A4DEB9A4C8A871AC,
    _:genid-6746439800084d48b9df2105733e82b8-4F424F06B9039F554F174524B8A30339;
  rdfs:comment "Validation constraint consisting of information about defined constraint."@en;
  rdfs:label "Validation constraint"@en .

:validationType a owl:DatatypeProperty;
  rdfs:comment "Type of validation: Error/Warning."@en;
  rdfs:label "validation type"@en;
  schema:domainIncludes :ValidationConstraint;
  schema:rangeIncludes xsd:string .

:validationUsecase a owl:DatatypeProperty;
  rdfs:comment "Use case for application of validation constraint wrt validating KM core Ontology or Data or DKM."@en;
  rdfs:label "validation use case"@en;
  schema:domainIncludes :ValidationConstraint;
  schema:rangeIncludes xsd:string .

:validationIntentDescription a owl:DatatypeProperty;
  rdfs:comment "Description of the test’s general intent (e.g. “validate correct range of each data property on any resource”)."@en;
  rdfs:label "validation intent description"@en;
  schema:domainIncludes :ValidationConstraint;
  schema:rangeIncludes xsd:string .

:validationLogicDescription a owl:DatatypeProperty;
  rdfs:comment "Description of the logic of the test (e.g.”IF data contains resource X with dataproperty P and value V of type T THEN ontology must define that the range of P includes type T or its supertype)."@en;
  rdfs:label "validation logic description"@en;
  schema:domainIncludes :ValidationConstraint;
  schema:rangeIncludes xsd:string .

:positiveTestCase a owl:DatatypeProperty;
  rdfs:comment "A snippet of RDF data expressed as a valid JSON-LD object or an RDF TriG document, which captures a relevant fragment of data addressed by the validation test, while satisfying its main condition."@en;
  rdfs:label "positive test case"@en;
  schema:domainIncludes :ValidationConstraint;
  schema:rangeIncludes xsd:string .

:negativeTestCase a owl:DatatypeProperty;
  rdfs:comment "A snippet of RDF data expressed as a valid JSON-LD object or an RDF TriG document, which captures a relevant fragment of data addressed by the validation test, while violating its main condition"@en;
  rdfs:label "negative test case"@en;
  schema:domainIncludes :ValidationConstraint;
  schema:rangeIncludes xsd:string .

:DataValidationConfig a owl:Class;
  rdfs:subClassOf owl:Thing, _:genid-6746439800084d48b9df2105733e82b8-AA44F46438A7087ACF9416C8B547DE85;
  rdfs:comment "Configuration for data validation test suite."@en;
  rdfs:label "Data validation configuration"@en .

:violatingResource1 a owl:ObjectProperty;
  rdfs:comment "violating resource 1 for violation data trace failing constraint."@en;
  rdfs:label "violating resource 1"@en;
  schema:domainIncludes :ViolatingDataTrace;
  schema:rangeIncludes owl:Thing .

:violatingResource2 a owl:ObjectProperty;
  rdfs:comment "violating resource 2 for violation data trace failing constraint."@en;
  rdfs:label "violating resource 2"@en;
  schema:domainIncludes :ViolatingDataTrace;
  schema:rangeIncludes owl:Thing .

:violatingResource3 a owl:ObjectProperty;
  rdfs:comment "violating resource 3 for violation data trace failing constraint."@en;
  rdfs:label "violating resource 3"@en;
  schema:domainIncludes :ViolatingDataTrace;
  schema:rangeIncludes owl:Thing .

:violatingResource4 a owl:ObjectProperty;
  rdfs:comment "violating resource 4 for violation data trace failing constraint."@en;
  rdfs:label "violating resource 4"@en;
  schema:domainIncludes :ViolatingDataTrace;
  schema:rangeIncludes owl:Thing .

:violatingResource5 a owl:ObjectProperty;
  rdfs:comment "violating resource 5 for violation data trace failing constraint."@en;
  rdfs:label "violating resource 5"@en;
  schema:domainIncludes :ViolatingDataTrace;
  schema:rangeIncludes owl:Thing .

:violatingResource6 a owl:ObjectProperty;
  rdfs:comment "violating resource 6 for violation data trace failing constraint."@en;
  rdfs:label "violating resource 6"@en;
  schema:domainIncludes :ViolatingDataTrace;
  schema:rangeIncludes owl:Thing .

:sparqlQueries a owl:ObjectProperty;
  rdfs:comment "Sparql query for validation of resources."@en;
  rdfs:label "SPARQL query"@en;
  schema:domainIncludes :DataValidationConfig;
  schema:rangeIncludes :SparqlQuery .

:similarityType a owl:DatatypeProperty;
  rdfs:comment "Similarity type applicable on attribute matcher."@en;
  rdfs:label "similarity type"@en;
  schema:domainIncludes :AttributeMatcher;
  schema:rangeIncludes xsd:string .

:handlerClassName a owl:DatatypeProperty;
  rdfs:comment "Name of handler class referenced in attribute matcher code base."@en;
  rdfs:label "handler class name"@en;
  schema:domainIncludes :AttributeMatcher;
  schema:rangeIncludes xsd:string .

:dependsOn a owl:ObjectProperty;
  rdfs:comment "Associates a dependent node with an independent node for effective mutation operations."@en;
  rdfs:label "depends on"@en;
  schema:domainIncludes owl:Thing .

:Kernel a owl:Class;
  rdfs:subClassOf owl:Thing, _:genid-6746439800084d48b9df2105733e82b8-392CFFD5BF59A1CCDBC903D047C37755;
  rdfs:comment "Software component having an input, output and configuration model intented for abstraction."@en;
  rdfs:label "Kernel"@en .

:Insight a owl:Class;
  rdfs:subClassOf owl:Thing;
  rdfs:comment "An insight is a runtime object created by fully configuring and instantiating a kernel."@en;
  rdfs:label "Insight"@en .

:DataDescriptor a owl:Class;
  rdfs:subClassOf owl:Thing;
  rdfs:comment "The class representing both inputs and outputs of insights."@en;
  rdfs:label "Data Descriptor"@en .

:DataStructure a owl:Class;
  rdfs:subClassOf owl:Thing;
  rdfs:comment "Data structures are supported abstract data types for input and output of insights (Scalar, Sequence, Set, Tabular and Tuple)."@en;
  rdfs:label "Data Structure"@en .

:ConfigurationItem a owl:Class;
  rdfs:subClassOf owl:Thing, _:genid-6746439800084d48b9df2105733e82b8-CB920E82075E905CFE466DCDE62707D7;
  rdfs:comment "Item in kernel configuration."@en;
  rdfs:label "Configuration Item"@en .

:ConfigurationItemValue a owl:Class;
  rdfs:subClassOf owl:Thing;
  rdfs:comment "Value for item in kernel configuration."@en;
  rdfs:label "Configuration Item Value"@en .

:hasInput a owl:ObjectProperty;
  rdfs:comment "Input for kernel."@en;
  rdfs:label "has kernel input"@en;
  schema:domainIncludes :Kernel;
  schema:rangeIncludes :DataDescriptor .

:hasOutput a owl:ObjectProperty;
  rdfs:comment "Output for kernel."@en;
  rdfs:label "has kernel output"@en;
  schema:domainIncludes :Kernel;
  schema:rangeIncludes :DataDescriptor .

:hasStructure a owl:ObjectProperty;
  rdfs:comment "Abstract datatype associated with kernel input/output."@en;
  rdfs:label "has structure"@en;
  schema:domainIncludes :DataDescriptor;
  schema:rangeIncludes :DataStructure .

:hasValueType a owl:ObjectProperty;
  rdfs:comment "Indicates the type applicable on item values."@en;
  rdfs:label "has value type"@en;
  schema:domainIncludes :ConfigurationItem .

:basedOn a owl:ObjectProperty;
  rdfs:comment "Associates an insight with the specific kernel used."@en;
  rdfs:label "based on"@en;
  schema:domainIncludes :Insight .

:forItem a owl:ObjectProperty;
  rdfs:comment "Value for configuration item."@en;
  rdfs:label "for item"@en;
  schema:domainIncludes :ConfigurationItemValue .

:hasConfigurationItem a owl:ObjectProperty;
  rdfs:comment "Item configured in kernel."@en;
  rdfs:label "has Configuration Item"@en;
  schema:domainIncludes :Insight .

:hasInsight a owl:ObjectProperty;
  rdfs:comment "Insights associated with an application."@en;
  rdfs:label "has insight"@en;
  schema:domainIncludes :Application .

:inputFrom a owl:ObjectProperty;
  rdfs:comment "Insight using defined insight."@en;
  rdfs:label "input from"@en;
  schema:domainIncludes :Insight .

:JsonData a owl:Class;
  rdfs:subClassOf :DataStructure .

:implementationClass a owl:DatatypeProperty;
  rdfs:comment "Classname having execution code for kernel."@en;
  rdfs:label "implementation class"@en;
  schema:domainIncludes :Kernel .

:Mention a owl:Class;
  rdfs:subClassOf owl:Thing;
  rdfs:comment "Provides metadata about extracted Entity/Relationship in KG."@en;
  rdfs:label "Mention"@en .

:mentionOf a owl:ObjectProperty;
  rdfs:comment "Associates Entity/Relationship with mention."@en;
  rdfs:label "mention of"@en;
  schema:domainIncludes :Mention .

:source a owl:ObjectProperty;
  rdfs:comment "Datasource from which mention is extracted."@en;
  rdfs:label "source"@en;
  schema:domainIncludes :Mention .

:ingestionTime a owl:DatatypeProperty;
  rdfs:comment "The time of persisting the mention in the KG."@en;
  rdfs:label "ingestion time"@en;
  schema:domainIncludes :Mention .

:fetchingTime a owl:DatatypeProperty;
  rdfs:comment "The time of fetching the mention from the source."@en;
  rdfs:label "fetching time"@en;
  schema:domainIncludes :Mention .

:sourceRefID a owl:DatatypeProperty;
  rdfs:comment "source reference id for entity/relationship."@en;
  rdfs:label "source ref id"@en;
  schema:domainIncludes :Entity, :Relationship .

_:genid-6746439800084d48b9df2105733e82b8-5BC5CB2EA85992929A61F7BDF2256141 a owl:Restriction;
  owl:onProperty :weight .

_:genid-6746439800084d48b9df2105733e82b8-2E9D3F7137F6A76B94974B7D76BF70F2 a owl:Restriction;
  owl:onProperty :cardinality .

_:genid-6746439800084d48b9df2105733e82b8-9746471FEBD076D53A5C77C697CBF4EC a owl:Restriction;
  owl:onProperty :isMandatory .

_:genid-6746439800084d48b9df2105733e82b8-382D61534EC133EFF603D88BCD44FF81 a owl:Restriction;
  owl:cardinality "1"^^xsd:nonNegativeInteger;
  owl:onProperty :enumerable .

_:genid-6746439800084d48b9df2105733e82b8-D11091805A807977944BCA0DB69B4C83 a owl:Restriction;
  owl:cardinality "1"^^xsd:nonNegativeInteger;
  owl:onProperty rdfs:label .

_:genid-6746439800084d48b9df2105733e82b8-11DEA6DD7E1795BBC455ED9F217BC4C0 a owl:Restriction;
  owl:cardinality "1"^^xsd:nonNegativeInteger;
  owl:onProperty :hasOwner .

_:genid-6746439800084d48b9df2105733e82b8-6D476D0F703404CEEFE0C18B304653F2 a owl:Restriction;
  owl:cardinality "1"^^xsd:nonNegativeInteger;
  owl:onProperty rdfs:label .

_:genid-6746439800084d48b9df2105733e82b8-49088FF45F25F3F99770047F6B347E2D a owl:Restriction;
  owl:cardinality "1"^^xsd:nonNegativeInteger;
  owl:onProperty :hasSchema .

_:genid-6746439800084d48b9df2105733e82b8-D639C7E3DA9990504771C273B2958348 a owl:Restriction;
  owl:cardinality "1"^^xsd:nonNegativeInteger;
  owl:onProperty :version .

_:genid-6746439800084d48b9df2105733e82b8-08AD7611C7ACAB54A6FD10D3820062E4 a owl:Restriction;
  owl:cardinality "1"^^xsd:nonNegativeInteger;
  owl:onProperty rdfs:label .

_:genid-6746439800084d48b9df2105733e82b8-4405AEBBDF958CEF1E7708B241281AEE a owl:Restriction;
  owl:cardinality "1"^^xsd:nonNegativeInteger;
  owl:onProperty :description .

_:genid-6746439800084d48b9df2105733e82b8-58D6840799894E91E9D5833215590993 a owl:Restriction;
  owl:cardinality "1"^^xsd:nonNegativeInteger;
  owl:onProperty :hasCatalog .

_:genid-6746439800084d48b9df2105733e82b8-87C9B026CF224FFE9F5E2FDA1DB42F75 a owl:Restriction;
  owl:cardinality "1"^^xsd:nonNegativeInteger;
  owl:onProperty :hasDKM .

_:genid-6746439800084d48b9df2105733e82b8-72DBE3ECD38BD00C9AB4E27BBFAD54A2 a owl:Restriction;
  owl:cardinality "1"^^xsd:nonNegativeInteger;
  owl:onProperty rdfs:label .

_:genid-6746439800084d48b9df2105733e82b8-F5CAC69CB0E4B3CFF7A6980E483298A0 a owl:Restriction;
  owl:cardinality "1"^^xsd:nonNegativeInteger;
  owl:onProperty rdfs:label .

_:genid-6746439800084d48b9df2105733e82b8-7371238C9EF20336A05A02C33FC95E25 a owl:Restriction;
  owl:cardinality "1"^^xsd:nonNegativeInteger;
  owl:onProperty :handlerClassName .

_:genid-6746439800084d48b9df2105733e82b8-ED6291985F77CB59B973D4E81D3F1D9A a owl:Restriction;
  owl:cardinality "1"^^xsd:nonNegativeInteger;
  owl:onProperty :similarityType .

_:genid-6746439800084d48b9df2105733e82b8-0B16489659A117A1E1002CF6235C797E a owl:Restriction;
  owl:cardinality "1"^^xsd:nonNegativeInteger;
  owl:onProperty :hasAttribute .

_:genid-6746439800084d48b9df2105733e82b8-2EEBDD89C16DE395ED765AFFFA896082 a owl:Restriction;
  owl:cardinality "1"^^xsd:nonNegativeInteger;
  owl:onProperty :credibility .

_:genid-6746439800084d48b9df2105733e82b8-0837DACF01C925857341BD806B158E86 a owl:Restriction;
  owl:cardinality "1"^^xsd:nonNegativeInteger;
  owl:onProperty :targetDomain .

_:genid-6746439800084d48b9df2105733e82b8-F1DB545944643BE6171516CCF3C1E0DB a owl:Restriction;
  owl:cardinality "1"^^xsd:nonNegativeInteger;
  owl:onProperty :hasOwner .

_:genid-6746439800084d48b9df2105733e82b8-DCC3D109A58A156AE0D95D2154E0402C a owl:Restriction;
  owl:cardinality "1"^^xsd:nonNegativeInteger;
  owl:onProperty :fetcherQuery, :overallCredibility .

_:genid-6746439800084d48b9df2105733e82b8-9F6026F57AD5C848E93F596D266B1946 a owl:Restriction;
  owl:cardinality "1"^^xsd:nonNegativeInteger;
  owl:onProperty :targetTerm .

_:genid-6746439800084d48b9df2105733e82b8-2FB2112B4CD459A620A61D4F4C9EFD34 a owl:Restriction;
  owl:cardinality "1"^^xsd:nonNegativeInteger;
  owl:onProperty :fetcherQueryParam .

_:genid-6746439800084d48b9df2105733e82b8-4B3BF59C37C21E83A64E0F4B77D91030 a owl:Restriction;
  owl:cardinality "1"^^xsd:nonNegativeInteger;
  owl:onProperty :paramValueAttribute .

_:genid-6746439800084d48b9df2105733e82b8-A377FED1B36A9F10C98F4CDA786715EB a owl:Restriction;
  owl:cardinality "1"^^xsd:nonNegativeInteger;
  owl:onProperty :queryString .

_:genid-6746439800084d48b9df2105733e82b8-65CDEC0784CC1FD612A5BD9E231F1E56 a owl:Restriction;
  owl:cardinality "1"^^xsd:nonNegativeInteger;
  owl:onProperty :tagValue .

_:genid-6746439800084d48b9df2105733e82b8-15D00213FFE7ED7AC14AEE7217507503 a owl:Restriction;
  owl:cardinality "1"^^xsd:nonNegativeInteger;
  owl:onProperty :tagKey .

_:genid-6746439800084d48b9df2105733e82b8-06F3D36FB458C9B9E7FABBF9AC02C5FD a owl:Restriction;
  owl:onProperty :referenceSource .

_:genid-6746439800084d48b9df2105733e82b8-61F8FBA8F30FFC8E0A12080541066628 a owl:Restriction;
  owl:cardinality "1"^^xsd:nonNegativeInteger;
  owl:onProperty :kgUsageCategory .

_:genid-6746439800084d48b9df2105733e82b8-7889BA61DF817F3F77DFA7ED239C51BC a owl:Restriction;
  owl:cardinality "1"^^xsd:nonNegativeInteger;
  owl:onProperty :hasOwner .

_:genid-6746439800084d48b9df2105733e82b8-599DAF6E1ECB4035C86ABF6DD80392AF a owl:Restriction;
  owl:cardinality "1"^^xsd:nonNegativeInteger;
  owl:onProperty :description .

_:genid-6746439800084d48b9df2105733e82b8-E4BFC45CCB15A51C1256CAED5FEE6199 a owl:Restriction;
  owl:onProperty :website .

_:genid-6746439800084d48b9df2105733e82b8-B2DE942CCE1B3BE4D2CAFF4B0C3F6DF6 a owl:Restriction;
  owl:cardinality "1"^^xsd:nonNegativeInteger;
  owl:onProperty rdfs:label .

_:genid-6746439800084d48b9df2105733e82b8-18219C53B0393C2DEA8647CCAFC74E8C a owl:Restriction;
  owl:cardinality "1"^^xsd:nonNegativeInteger;
  owl:onProperty :dataValidityPeriodInHours .

_:genid-6746439800084d48b9df2105733e82b8-C4BD601677F153FEA84A8FA729D66EC9 a owl:Restriction;
  owl:cardinality "1"^^xsd:nonNegativeInteger;
  owl:onProperty :sourceMedium .

_:genid-6746439800084d48b9df2105733e82b8-CB920E82075E905CFE466DCDE62707D7 a owl:Restriction;
  owl:cardinality "1"^^xsd:nonNegativeInteger;
  owl:onProperty rdfs:label .

_:genid-6746439800084d48b9df2105733e82b8-4805876D8198EFD31220D0C776C766B2 a owl:Restriction;
  owl:cardinality "1"^^xsd:nonNegativeInteger;
  owl:onProperty :endpointURL .

_:genid-6746439800084d48b9df2105733e82b8-60274FBC857B96C997097A6B734DB8B7 a owl:Restriction;
  owl:cardinality "1"^^xsd:nonNegativeInteger;
  owl:onProperty :paginationMode .

_:genid-6746439800084d48b9df2105733e82b8-1CEBA1321A0DC87AAE75E5731D08E463 a owl:Restriction;
  owl:cardinality "1"^^xsd:nonNegativeInteger;
  owl:onProperty :responsePattern .

_:genid-6746439800084d48b9df2105733e82b8-083164EC1D5A7192C343F2E5092C2AF4 a owl:Restriction;
  owl:cardinality "1"^^xsd:nonNegativeInteger;
  owl:onProperty :maxParallelism .

_:genid-6746439800084d48b9df2105733e82b8-9197CED36C10EF78061BF49136C19BD6 a owl:Restriction;
  owl:cardinality "1"^^xsd:nonNegativeInteger;
  owl:onProperty :serves .

_:genid-6746439800084d48b9df2105733e82b8-392CFFD5BF59A1CCDBC903D047C37755 a owl:Restriction;
  owl:cardinality "1"^^xsd:nonNegativeInteger;
  owl:onProperty :implementationClass .

_:genid-6746439800084d48b9df2105733e82b8-00F064439EC626D99F909E28643CC94E a owl:Restriction;
  owl:onProperty :hasRange .

_:genid-6746439800084d48b9df2105733e82b8-02A0499502B45FD7003F68DE85CF9E85 a owl:Restriction;
  owl:onProperty :hasDomain .

_:genid-6746439800084d48b9df2105733e82b8-F4DEE88442E4A64EE808B149579972F9 a owl:Restriction;
  owl:onProperty :referenceTerm .

_:genid-6746439800084d48b9df2105733e82b8-95B9566C26265D611AD436E2EF19B40B a owl:Restriction;
  owl:cardinality "1"^^xsd:nonNegativeInteger;
  owl:onProperty rdfs:label .

_:genid-6746439800084d48b9df2105733e82b8-8BFC629C1BA2ED077BD0164116ECA14B a owl:Restriction;
  owl:cardinality "1"^^xsd:nonNegativeInteger;
  owl:onProperty :validationType .

_:genid-6746439800084d48b9df2105733e82b8-23C63E89CD7FE84E5A97DC2EF50F1946 a owl:Restriction;
  owl:cardinality "1"^^xsd:nonNegativeInteger;
  owl:onProperty :validationUsecase .

_:genid-6746439800084d48b9df2105733e82b8-5AF5774FDED6F78E18507AECA5026364 a owl:Restriction;
  owl:cardinality "1"^^xsd:nonNegativeInteger;
  owl:onProperty :validationIntentDescription .

_:genid-6746439800084d48b9df2105733e82b8-54BBD6EB4E58ADBB939DEB1EB4B920AD a owl:Restriction;
  owl:cardinality "1"^^xsd:nonNegativeInteger;
  owl:onProperty :validationLogicDescription .

_:genid-6746439800084d48b9df2105733e82b8-7131B58332CB5918A4DEB9A4C8A871AC a owl:Restriction;
  owl:cardinality "1"^^xsd:nonNegativeInteger;
  owl:onProperty :positiveTestCase .

_:genid-6746439800084d48b9df2105733e82b8-4F424F06B9039F554F174524B8A30339 a owl:Restriction;
  owl:cardinality "1"^^xsd:nonNegativeInteger;
  owl:onProperty :negativeTestCase .

_:genid-6746439800084d48b9df2105733e82b8-1AED1946F64D34E5E6D120CCF23E2983 a owl:Restriction;
  owl:cardinality "1"^^xsd:nonNegativeInteger;
  owl:onProperty rdfs:comment .

_:genid-6746439800084d48b9df2105733e82b8-DB16376A000F45392A86C60D792C65C0 a owl:Restriction;
  owl:cardinality "1"^^xsd:nonNegativeInteger;
  owl:onProperty :constraint .

_:genid-6746439800084d48b9df2105733e82b8-535BEB1DC0EBB47191057BAA3DA7D606 a owl:Restriction;
  owl:cardinality "1"^^xsd:nonNegativeInteger;
  owl:onProperty :violatingData .

_:genid-6746439800084d48b9df2105733e82b8-07FD9ADD00D292940971899CF952175B a owl:Restriction;
  owl:cardinality "1"^^xsd:nonNegativeInteger;
  owl:onProperty :inGraph .

_:genid-6746439800084d48b9df2105733e82b8-9E7542BA53AF77F7692A3F18B731D669 a owl:Restriction;
  owl:cardinality "1"^^xsd:nonNegativeInteger;
  owl:onProperty :violatingResource1 .

_:genid-6746439800084d48b9df2105733e82b8-A27BB97FFA10B3E76266C4A3EB38FCC4 a owl:Restriction;
  owl:onProperty :violatingResource2 .

_:genid-6746439800084d48b9df2105733e82b8-29B28C7FF7BBE4CF7213CEBA161202ED a owl:Restriction;
  owl:onProperty :violatingResource3 .

_:genid-6746439800084d48b9df2105733e82b8-08F26CB98CC0FAB64C8B28FC490E134B a owl:Restriction;
  owl:onProperty :violatingResource4 .

_:genid-6746439800084d48b9df2105733e82b8-489EB08BF2372314A349F48EB396FB4F a owl:Restriction;
  owl:onProperty :violatingResource5 .

_:genid-6746439800084d48b9df2105733e82b8-BFB5A9BF98D939D3BDBAC7894F044580 a owl:Restriction;
  owl:onProperty :violatingResource6 .

_:genid-6746439800084d48b9df2105733e82b8-AA44F46438A7087ACF9416C8B547DE85 a owl:Restriction;
  owl:cardinality "1"^^xsd:nonNegativeInteger;
  owl:onProperty :sparqlQueries .

_:genid-6746439800084d48b9df2105733e82b8-A0595A7A894762C7B2E34E4DA362D4DB a owl:Restriction;
  owl:onProperty :hasAttributeCredibility .

_:genid-6746439800084d48b9df2105733e82b8-D57C776D9DD739700E2EE756A03D22E6 a owl:Restriction;
  owl:cardinality "1"^^xsd:nonNegativeInteger .

_:genid-6746439800084d48b9df2105733e82b8-E28BE85183794D5489754787A6AD493C a owl:Restriction;
  owl:cardinality "1"^^xsd:nonNegativeInteger;
  owl:onProperty :referenceSource .

_:genid-6746439800084d48b9df2105733e82b8-5759C29233FBAF0830889A9FDBEC96EB a owl:Restriction;
  owl:cardinality "1"^^xsd:nonNegativeInteger;
  owl:onProperty rdfs:label .

:basedOn schema:rangeIncludes :Kernel .

:forItem schema:rangeIncludes :ConfigurationItem .

:hasConfigurationItem schema:rangeIncludes :ConfigurationItemValue .

:hasInsight schema:rangeIncludes :Insight .

:inputFrom schema:rangeIncludes :Insight .

:implementationClass schema:rangeIncludes xsd:string .

:mentionOf schema:rangeIncludes :Entity, :Relationship .

:source schema:rangeIncludes :Entity, :Relationship .

:ingestionTime schema:rangeIncludes xsd:dateTime .

:fetchingTime schema:rangeIncludes xsd:dateTime .

:sourceRefID schema:rangeIncludes xsd:string .

_:genid-6746439800084d48b9df2105733e82b8-A0595A7A894762C7B2E34E4DA362D4DB owl:minCardinality
    "1"^^xsd:nonNegativeInteger .
